theories/IL/NoParams.v
@@ -1,0 +1,21 @@
+Require Import IL.
+
+Inductive noParams : stmt->Prop :=
+| NoParamsLet
+    x e s
+    (NoParamsIH:noParams s)
+    : noParams (stmtLet x e s)
+| NoParamsIf
+    e s t
+    (NoParamsIH1:noParams s)
+    (NoParamsIH2:noParams t)
+  : noParams (stmtIf e s t)
+| NoParamsApp l :
+   noParams (stmtApp l nil)
+| NoParamsExp e :
+    noParams (stmtReturn e)
+| NoParamsCall F t
+  (NoParamsIHF:forall n Zs, get F n Zs -> noParams (snd Zs))
+  (NoParamsF:forall n Zs, get F n Zs -> fst Zs = nil)
+  (NoParamsIHt:noParams t)
+  : noParams (stmtFun F t).
